base cases; Fixpoint; all same k for now

coq/two/LambdaTwo.v
@@ -1,79 +1,39 @@
 Require Export LambdaTwoSyntax.
 Require Export IndistinguishabilityTwo.
 
-Reserved Notation "[ L , P ] pc ; e ⊢ t ⇓ a" (at level 70).
-Inductive eval :
-  two -> (value -> value -> Prop) ->
-  two -> env -> term -> option atom -> Prop :=
 
-| E_Nat : forall L P pc e n,
-(* ------------------------------------------------------ *)
-    [L, P] pc; e ⊢ TNat n ⇓ Some (Atom (VNat n) pc)
-
-| E_Var : forall L P pc e n v l,
-    atIndex e n = Some (Atom v l) ->
-(* ------------------------------------------------------ *)
-    [L, P] pc; e ⊢ TVar n ⇓ Some (Atom v (l ⊔ pc))
-
-| E_Abs : forall L P pc e t,
-(* ------------------------------------------------------ *)
-    [L, P] pc; e ⊢ TLam t ⇓ Some (Atom (VClos e t) pc)
-
-| E_App : forall L P pc e t1 t2 e1' t1' l1 a2 a3,
-    [L, P] pc; e ⊢ t1 ⇓ Some (Atom (VClos e1' t1') l1) ->
-    [L, P] pc; e ⊢ t2 ⇓ Some a2 ->
-    [L, P] l1; a2 :: e1' ⊢ t1' ⇓ Some a3 ->
-(* ------------------------------------------------------ *)
-    [L, P] pc; e ⊢ TApp t1 t2 ⇓ Some a3
-
-(*| E_App1 : forall L P pc e t1 t2,
-    [L, P] pc; e ⊢ t1 ⇓ None ->
-(* ------------------------------------------------------ *)
-    [L, P] pc; e ⊢ TApp t1 t2 ⇓ None*)
-
-(*| E_App2 : forall L P pc e t1 t2, 
-    [L, P] pc; e ⊢ t2 ⇓ None ->
-(* ------------------------------------------------------ *)
-    [L, P] pc; e ⊢ TApp t1 t2 ⇓ None*)
-
-(*| E_App3 : forall L P pc e t1 t2 e1' t1' l1 a2,
-    [L, P] pc; e ⊢ t1 ⇓ Some (Atom (VClos e1' t1') l1) ->
-    [L, P] pc; e ⊢ t2 ⇓ Some a2 ->
-    [L, P] l1; a2 :: e1' ⊢ t1' ⇓ None ->
-(* ------------------------------------------------------ *)
-    [L, P] pc; e ⊢ TApp t1 t2 ⇓ None*)
-
-| E_Decl1 : forall L P pc e t1 t2 v,
-    [L, P] pc; e ⊢ TApp t1 t2 ⇓ Some (Atom v Bottom2) ->
-(* ------------------------------------------------------ *)
-    [L, P] pc; e ⊢ TDecl t1 t2 ⇓ Some (Atom v Bottom2)
-
-(*| E_Decl : forall L P pc e t1 t2,
-    [L, P] pc; e ⊢ TApp t1 t2 ⇓ None ->
-(* ------------------------------------------------------ *)
-    [L, P] pc; e ⊢ TDecl t1 t2 ⇓ None*)
-
-| E_Decl2 : forall L P pc e t1 t2 e1' t1' l1 a2 v3,
-    [L, P] pc; e ⊢ t1 ⇓ Some (Atom (VClos e1' t1') l1) ->
-    [L, P] pc; e ⊢ t2 ⇓ Some a2 ->
-    [L, P] l1; a2 :: e1' ⊢ t1' ⇓ Some (Atom v3 Top2) ->
-    forall a2' e2' v3',
-      env_LPequiv L P (a2 :: e1') (a2' :: e2') ->
-      [L, P] l1; a2' :: e2' ⊢ t1' ⇓ Some (Atom v3' Top2) ->
-      value_LPequiv L P v3 v3' ->
-(* ------------------------------------------------------ *)
-    [L, P] pc; e ⊢ TDecl t1 t2 ⇓ Some (Atom v3 Bottom2)
-
-| E_Decl21 : forall L P pc e t1 t2 e1' t1' l1 a2 v3,
-    [L, P] pc; e ⊢ t1 ⇓ Some (Atom (VClos e1' t1') l1) ->
-    [L, P] pc; e ⊢ t2 ⇓ Some a2 ->
-    [L, P] l1; a2 :: e1' ⊢ t1' ⇓ Some (Atom v3 Top2) ->
-    forall a2' e2',
-      env_LPequiv L P (a2 :: e1') (a2' :: e2') ->
-      [L, P] l1; a2' :: e2' ⊢ t1' ⇓ None ->
-(* ------------------------------------------------------ *)
-    [L, P] pc; e ⊢ TDecl t1 t2 ⇓ Some (Atom v3 Bottom2)
-
-where "[ L , P ] pc ; e ⊢ t ⇓ a" := (eval L P pc e t a).
-
-Hint Constructors eval.
+Fixpoint eval L P pc e t a k {struct k} : Prop :=
+  match t, k with
+    | TNat n, 0 =>
+      a = Atom (VNat n) pc
+    | TVar n, 0 =>
+      match atIndex e n with
+        | Some (Atom v l) =>
+          a = Atom v (l ⊔ pc)
+        | None => False
+      end
+    | TLam t', 0 =>
+      a = Atom (VClos e t') pc
+    | TApp t1 t2, S k' =>
+      forall e1' t1' l1 a2 a3,
+        eval L P pc e t1 (Atom (VClos e1' t1') l1) k' ->
+        eval L P pc e t2 a2 k' ->
+        eval L P l1 (a2 :: e1') t1' a3 k' ->
+        a = a3
+    | TDecl t1 t2, S k' =>
+      forall e1' t1' l1 a2 a3,
+        eval L P pc e t1 (Atom (VClos e1' t1') l1) k' ->
+        eval L P pc e t2 a2 k' ->
+        eval L P l1 (a2 :: e1') t1' a3 k' ->
+        match a3 with
+          | Atom v3 Bottom2 =>
+            a = a3
+          | Atom v3 Top2 =>
+            (forall a2' e2' v3',
+               env_LPequiv L P (a2 :: e1') (a2' :: e2') ->
+               eval L P l1 (a2' :: e2') t1' (Atom v3' Top2) k' ->
+               value_LPequiv L P v3 v3') ->
+            a = Atom v3 Bottom2
+        end
+    | _, _ => False
+  end.
